\documentclass{article}
\usepackage[utf8]{inputenc}

\title{Fibonacci and Useless Graphs}
\author{Justin Baum}
\date{March 5, 2018 - May 31 2018}

\usepackage{natbib}
\usepackage{graphicx}
\usepackage{seqsplit}
\usepackage{amssymb}
\usepackage{amsmath}
\usepackage{amsthm}


\newtheorem{theorem}{Theorem}[section]
\newtheorem{corollary}{Corollary}[theorem]
\newtheorem{lemma}[theorem]{Lemma}



\begin{document}

\maketitle

\section{Introduction}
We make a graph with the fibonacci sequence where each node is a number in the sequence, and every edge is any two nodes that when multiplied and subtracted with another(any node), give us another number in the fibonacci sequence. Then a set containing 1,2,3. We get some probably useless but neat properties.
\[S=\{a_{1}=1;a_{2}=1; a_{n}=a_{n-1}+a_{n-2}|n\in \mathbb{N}\}\]
\[V(G)=S\]
\[ij\in E(G)\leftrightarrow (i \in S \wedge j \in S \wedge ((\exists k \in S)(i\cdot j-k\in S))\]
\[Q=\{1,2,3\}\]
\section{Conjectures}
Conjecture 1: \[(\forall i \in S)(\forall j \in S)((i\in Q \vee j\in Q) \wedge (i \neq 1 \vee j \neq 1) \rightarrow ij \in E(G)\]
Conjecture 2: \[(\forall i \in S)(\forall j \in S)(i\notin Q \wedge j\notin Q \rightarrow ij \notin E(G))\]


\begin{lemma}
  \[(\forall i \in S)(\forall j \in S)((i\in Q \vee j\in Q) \wedge (i \neq 1 \vee j \neq 1) \rightarrow ij \in E(G)\]
  \begin{proof}i=1\\
    Want: ${\{1,j\} \in S}$\newline
    Need: ${j-k \in S}$
    \begin{enumerate}
        \item ${j = a_{n}}\because j \in S$
        \item ${j-k}$
        \item ${a_{n}-k}$
        \item ${a_{n-1}+a_{n-2}-k}$
        \item ${let\ k=a_{n-2}}\because k \in S$
        \item ${j-k=a_{n-1}+a_{n-2}-a_{n-1}=a_{n-1}}$
        \item ${a_{n-1}\in S}$
        \item $\therefore {(\forall j \in S)(\exists k \in S)(j-k \in S) \rightarrow (\forall j \in S) (\{1,j\} \in E(G))}$
    \end{enumerate}
  \end{proof}
  \begin{proof}i=2\\
    Want: ${\{2,j\} \in S}$\newline
    Need: ${2j-k \in S}$
    \begin{enumerate}
        \item ${j=a_{n}}\because j \in S$
        \item ${2j-k}$
        \item ${2a_{n}-k}$
        \item ${let\  k=a_{n}}\because k \in S$
        \item ${2j-k=2a_{n}-a_{n}=a_{n}}$
        \item $\therefore{(\forall j \in S)(\exists k \in S)(2j-k \in S)\rightarrow(\forall j)(\{2,j\}\in E(G))}$
    \end{enumerate}
  \end{proof}
  \begin{proof} i=3\\
    Want: ${\{3,j\} \in S}$\newline
    Need: ${3j-k \in S}$
    \begin{enumerate}
        \item ${j=a_{n}}\because j\in S$
        \item ${3j-k}$
        \item ${3a_{n}-k}$
        \item ${3a_{n-1}+3a_{n-2}-k}$
        \item ${3a_{n-2}+3a_{n-3}+3a_{n-2}-k}$
        \item ${6a_{n-2}+3a_{n-2}-k}$
        \item ${let\  k = a_{n-2}}\because k \in S$
        \item ${5a_{n-2}+3_a{n-3}}$
        \item ${3(a_{n-2}+a_{n-3})+2a_{n-2}}$
        \item ${3a_{n-1}+2a_{n-2}}$
        \item ${2(a_{n-1}+a_{n-2})+a_{n-1}}$
        \item ${2a_{n}+a_{n-1}}$
        \item ${(a_{n}+a_{n-1})+a_{n}}$
        \item ${a_{n+1} + a_{n}}$
        \item ${a_{n+2}}$
        \item $\therefore {(\forall j \in S)(\exists k \in S)(3j-k \in S)\rightarrow(\forall j\in S)(\{3,j\}\in E(G))}$
    \end{enumerate}
  \end{proof}
\end{lemma}

\section{Conjecture 2: Exhaustive Search}
For a finite universe of the first 45 terms of the fibonacci sequence:\\
\[|E(G)|=128\]
The second conjecture on these results also remained true.\\
I also ran a test through the first 1000 terms, and the second conjecture held true. However this is not a proof, and my professor Dr. Cooper believes I need to hash out some number theory to fully prove this conjecture.
\section{Conclusion}
Useless graph with neat properties, the second conjecture most likely needs some number theory, so hopefully this is completed at some point. I was unable to find any papers with this conjecture, but then again I only used Google Scholar.
\bibliographystyle{plain}
\bibliography{references}
\end{document}
